#
#  Copyright © 2011-2012 BiKE, SNU. All Rights Reserved.
#
#  This work is licensed under the Creative Commons Attribution 3.0 Unported License.
#  To view a copy of this license, visit http://creativecommons.org/licenses/by/3.0/
#  or send a letter to Creative Commons, 444 Castro Street, Suite 900, Mountain View,
#  California, 94041, USA.
#
#  This copyright applies only to the CDT Ontology Specification and accompanying
#  documentation in RDF; it does not apply to CDT data formats, ontology terms, or
#  technology. Regarding underlying technology, CDT relies heavily on W3C's RDF
#  technology, an open Web standard that can be freely used by anyone.
#

@prefix xsd: <http://www.w3.org/2001/XMLSchema#> .
@prefix rdfs: <http://www.w3.org/2000/01/rdf-schema#> .
@prefix owl: <http://www.w3.org/2002/07/owl#> .
@prefix adms: <http://www.w3.org/ns/adms#> .
@prefix vann: <http://purl.org/vocab/vann/> .
@prefix vs: <http://www.w3.org/2003/06/sw-vocab-status/ns#> .
@prefix dcterms: <http://purl.org/dc/terms/> .
@prefix foaf: <http://xmlns.com/foaf/0.1/> .
@prefix cdt: <http://vocab.bike.re.kr/cdt#> .

# OWL 2 DL Compliance Statements ###############################################

adms:SemanticAsset a owl:Class ;
  rdfs:isDefinedBy <http://www.w3.org/ns/adms> .
adms:status a owl:ObjectProperty ;
  rdfs:isDefinedBy <http://www.w3.org/ns/adms> .
dcterms:type a owl:ObjectProperty ;
    rdfs:isDefinedBy <http://purl.org/dc/terms/> .
dcterms:description a owl:DatatypeProperty ;
  rdfs:isDefinedBy <http://purl.org/dc/terms/> .
dcterms:publisher a owl:ObjectProperty ;
  rdfs:isDefinedBy <http://purl.org/dc/terms/> .
dcterms:license a owl:ObjectProperty ;
  rdfs:isDefinedBy <http://purl.org/dc/terms/> .
foaf:Person a owl:Class ;
  rdfs:isDefinedBy <http://xmlns.com/foaf/0.1/> .
foaf:Organization a owl:Class ;
  rdfs:isDefinedBy <http://xmlns.com/foaf/0.1/> .
foaf:name a owl:DatatypeProperty ;
  rdfs:isDefinedBy <http://xmlns.com/foaf/0.1/> .
foaf:mbox_sha1sum a owl:DatatypeProperty ;
  rdfs:isDefinedBy <http://xmlns.com/foaf/0.1/> .
foaf:homepage a owl:ObjectProperty ;
  rdfs:isDefinedBy <http://xmlns.com/foaf/0.1/> .
foaf:member a owl:ObjectProperty ;
  rdfs:isDefinedBy <http://xmlns.com/foaf/0.1/> .

# Ontology #####################################################################

<http://vocab.bike.re.kr/cdt> a owl:Ontology , adms:SemanticAsset ;
  dcterms:title "CDT Ontology"@en ;
  dcterms:description """
    CDT (Clinical Document Template) Ontology is an ontology for
    describing both structural and semantics-based clinical knowledge embedded
    in the level of clinical document templates. You can always find the latest
    version of the ontology at: https://github.com/SNUBiKE/CDT-Ontology
    """@en ;
  rdfs:seeAlso <https://github.com/SNUBiKE/CDT-Ontology> ;
  dcterms:creator [
      a foaf:Person ;
      owl:sameAs <http://bike.re.kr/id/people/sjnam> ;
      foaf:name "Sejin Nam"@en , "남세진"@ko ;
      foaf:mbox_sha1sum "b413a63576e5baf0f1785ea090420586265dc848"
    ] , [
      a foaf:Person ;
      owl:sameAs <http://bike.re.kr/id/people/jgkim> , <http://jayg.me/> ;
      foaf:name "James G. Kim"@en , "김보람"@ko ;
      foaf:mbox_sha1sum "a637717b7e34b83694018e8fdd3ff334fffcd4f3" ;
      foaf:homepage <http://jayg.org/>
    ] ;
  dcterms:publisher [
      a foaf:Organization ;
      owl:sameAs <http://bike.re.kr/id/bike> ;
      foaf:name "BiKE, SNU"@en ;
      dcterms:title "Biomedical Knowledge Engineering Laboratory, Seoul National University"@en ;
      foaf:mbox_sha1sum "aba4ca3a6825fc773570932dba553d95e9209e91" ;
      foaf:homepage <http://bike.re.kr/> , <http://bike.snu.ac.kr/> ;
      foaf:member <http://bike.re.kr/id/people/sjnam> , <http://bike.re.kr/id/people/jgkim>
    ] ;
  vann:preferredNamespaceUri "http://vocab.bike.re.kr/cdt#" ;
  vann:preferredNamespacePrefix "cdt" ;
  dcterms:type <http://purl.org/adms/assettype/Ontology> ;
  adms:status <http://purl.org/adms/status/UnderDevelopment> ;
  dcterms:license <http://creativecommons.org/licenses/by/3.0/> ;
  dcterms:created "2011-12-20+09:00"^^xsd:date ;
  dcterms:modified "2012-07-22+09:00"^^xsd:date ;
  owl:versionInfo "0.5" .

# Classes #####################################################################

cdt:ClinicalDocumentTemplate a owl:Class ;
  rdfs:label "Clinical Document Template"@en ;
  rdfs:comment """
    A Clinical Document Template (CDT) is a container for the content of a
    clinical document.
    """@en ;
  rdfs:isDefinedBy <http://vocab.bike.re.kr/cdt> ;
  vs:term_status "testing"@en .

cdt:TemplateComponent a owl:Class ;
  rdfs:label "Template Component"@en ;
  rdfs:comment """
    A Template Component is something that can be in a clinical document
    template.
    """@en ;
  rdfs:isDefinedBy <http://vocab.bike.re.kr/cdt> ;
  vs:term_status "unstable"@en .

cdt:TemplateDescriptionEntity a owl:Class ;
  rdfs:subClassOf cdt:TemplateComponent ;
  rdfs:label "Template Description Entity"@en ;
  rdfs:comment """
    A Template Description Entity (TDE) is a data entity holding a key/value
    pair in a clinical document template.
    """@en ;
  rdfs:isDefinedBy <http://vocab.bike.re.kr/cdt> ;
  vs:term_status "testing"@en .

cdt:Relation a owl:Class ;
  rdfs:label "Relation"@en ;
  rdfs:comment """
    Relation is a meta concept that subsumes the different types of binary or
    n-ary relations that can be defined.
    """@en ;
  rdfs:isDefinedBy <http://vocab.bike.re.kr/cdt> ;
  vs:term_status "unstable"@en .

cdt:CDTRelation a owl:Class ;
  rdfs:subClassOf cdt:Relation ;
  rdfs:label "CDT Relation"@en ;
  rdfs:comment """
    A CDT Relation is a relation from template components to clinical document
    templates.
    """@en ;
  rdfs:isDefinedBy <http://vocab.bike.re.kr/cdt> ;
  vs:term_status "unstable"@en .

cdt:TDERelation a owl:Class ;
  rdfs:subClassOf cdt:Relation ;
  rdfs:subClassOf cdt:TemplateComponent ;
  rdfs:label "TDE Relation"@en ;
  rdfs:comment """
    A TDE Relation is a relation among template description entities.
    """@en ;
  rdfs:isDefinedBy <http://vocab.bike.re.kr/cdt> ;
  vs:term_status "unstable"@en .

cdt:UsedAtRelation a owl:Class ;
  rdfs:subClassOf cdt:CDTRelation ;
  rdfs:label "UsedAt Relation"@en ;
  rdfs:comment """
    A UsedAt Relation is a CDT relation that represents usage of template
    components in clinical document templates.
    """@en ;
  rdfs:isDefinedBy <http://vocab.bike.re.kr/cdt> ;
  vs:term_status "unstable"@en .

cdt:ContainRelation a owl:Class ;
  rdfs:subClassOf cdt:TDERelation ;
  rdfs:label "Contain Relation"@en ;
  rdfs:comment """
    A Contain Relation is a TDE relation that represents inclusion of
    template description entities.
    """@en ;
  rdfs:isDefinedBy <http://vocab.bike.re.kr/cdt> ;
  vs:term_status "unstable"@en .

cdt:AdjacentToRelation a owl:Class ;
  rdfs:subClassOf cdt:TDERelation ;
  rdfs:label "AdjacentTo Relation"@en ;
  rdfs:comment """
    A AdjacentTo Relation is a TDE relation that represents dispositional
    nextness of template description entities.
    """@en ;
  rdfs:isDefinedBy <http://vocab.bike.re.kr/cdt> ;
  vs:term_status "unstable"@en .

cdt:Constraint a owl:Class ;
  rdfs:label "Constraint"@en ;
  rdfs:comment """
    A Constraint is a concept that defines a range of values a template
    description entity can posesses, or specifies generic constraints among
    template description entities.
    """@en ;
  rdfs:isDefinedBy <http://vocab.bike.re.kr/cdt> ;
  vs:term_status "unstable"@en .

cdt:Context a owl:Class ;
  rdfs:label "Context"@en ;
  rdfs:comment """
    A Context is a concept that represents circumstances in which a template
    description entity appears.
    """@en ;
  rdfs:isDefinedBy <http://vocab.bike.re.kr/cdt> ;
  vs:term_status "unstable"@en .

# Properties ##################################################################

cdt:source a owl:ObjectProperty ;
  rdfs:domain cdt:Relation ;
  rdfs:label "source"@en ;
  rdfs:comment """
    Links to an instance that is a source or origin of the directed binary
    or n-ary relation.
    """@en ;
  rdfs:isDefinedBy <http://vocab.bike.re.kr/cdt> ;
  vs:term_status "unstable"@en .

cdt:target a owl:ObjectProperty ;
  rdfs:domain cdt:Relation ;
  rdfs:label "target"@en ;
  rdfs:comment """
    Links to an instance that is a target of the directed binary or n-ary
    relation.
    """@en ;
  rdfs:isDefinedBy <http://vocab.bike.re.kr/cdt> ;
  vs:term_status "unstable"@en .

cdt:constraint a owl:ObjectProperty ;
  rdfs:domain cdt:TemplateDescriptionEntity ;
  rdfs:range cdt:Constraint ;
  rdfs:label "constraint"@en ;
  rdfs:comment """
    Links to a constraint the template description entity has.
    """@en ;
  rdfs:isDefinedBy <http://vocab.bike.re.kr/cdt> ;
  vs:term_status "unstable"@en .

cdt:context a owl:ObjectProperty ;
  rdfs:domain cdt:TemplateDescriptionEntity ;
  rdfs:range cdt:Context ;
  rdfs:label "context"@en ;
  rdfs:comment """
    Links to a context in which the template description entity appears.
    """@en ;
  rdfs:isDefinedBy <http://vocab.bike.re.kr/cdt> ;
  vs:term_status "unstable"@en .

cdt:department a owl:DatatypeProperty ;
  rdfs:domain cdt:ClinicalDocumentTemplate ;
  rdfs:range rdfs:Literal ;
  rdfs:label "department"@en ;
  rdfs:comment """
    The department where the clinical document template is defined and used.
    """@en ;
  rdfs:isDefinedBy <http://vocab.bike.re.kr/cdt> ;
  vs:term_status "archaic"@en .

cdt:filename a owl:DatatypeProperty ;
  rdfs:domain cdt:ClinicalDocumentTemplate ;
  rdfs:range rdfs:Literal ;
  rdfs:label "filename"@en ;
  rdfs:comment """
    The name of the file in which the clinical document template is stored.
    """@en ;
  rdfs:isDefinedBy <http://vocab.bike.re.kr/cdt> ;
  vs:term_status "archaic"@en .

dcterms:references a owl:ObjectProperty ;
  rdfs:label "references"@en ;
  rdfs:comment """
    The dcterms:references property fully represents the CDT Ontology
    relationship of the same name. The CDT Ontology uses this to link to a
    related resource that is referenced, cited, or otherwise pointed to by the
    described template description entity.
    """@en ;
  rdfs:isDefinedBy <http://purl.org/dc/terms/> .

dcterms:title a owl:DatatypeProperty ;
  rdfs:label "title"@en ;
  rdfs:comment """
    The dcterms:title property fully represents the CDT Ontology property of
    name that is used to describe a name given to the instance in the ontology.
    """@en ;
  rdfs:isDefinedBy <http://purl.org/dc/terms/> .

dcterms:creator a owl:ObjectProperty ;
  rdfs:label "creator"@en ;
  rdfs:comment """
    The dcterms:creator property fully represents the CDT Ontology property of
    the same name. The CDT Ontology uses this to link to an agent responsible
    for making the instance in the ontology.
    """@en ;
  rdfs:isDefinedBy <http://purl.org/dc/terms/> .

dcterms:created a owl:DatatypeProperty ;
  rdfs:label "created"@en ;
  rdfs:comment """
    The dcterms:created property fully represents the CDT Ontology property of
    the same name. The CDT Ontology uses this to describe the date of creation
    of the instance in the ontology.
    """@en ;
  rdfs:isDefinedBy <http://purl.org/dc/terms/> .

dcterms:modified a owl:DatatypeProperty ;
  rdfs:label "modified"@en ;
  rdfs:comment """
    The dcterms:modified property fully represents the CDT Ontology property of
    the same name. The CDT Ontology uses this to describe the date on which the
    instance in the ontology was changed.
    """@en ;
  rdfs:isDefinedBy <http://purl.org/dc/terms/> .

# Restrictions ################################################################

cdt:CDTRelation rdfs:subClassOf [
    a owl:Restriction ;
    owl:onProperty cdt:source ;
    owl:allValuesFrom cdt:TemplateComponent
  ] , [
    a owl:Restriction ;
    owl:onProperty cdt:target ;
    owl:allValuesFrom cdt:ClinicalDocumentTemplate
  ] .

cdt:TDERelation rdfs:subClassOf [
    a owl:Restriction ;
    owl:onProperty cdt:source ;
    owl:allValuesFrom cdt:TemplateDescriptionEntity
  ] , [
    a owl:Restriction ;
    owl:onProperty cdt:target ;
    owl:allValuesFrom cdt:TemplateDescriptionEntity
  ] .